FormalSystem/FrameConditions/Soundness.lean
@@ -4,6 +4,7 @@ Released under Apache 2.0 license as described in the file LICENSE.
 Authors: Benjamin Brast-McKie
 -/
 
+import FormalSystem.FrameConditions.FrameClass
 import FormalSystem.FrameConditions.Validity
 import FormalSystem.Metalogic.Soundness
 
